MirrorCharge!/src/MirrorCharge/Java/Semantics.v
@@ -17,7 +17,6 @@ Require Import ExtLib.Data.PreFun.
 Require Import ExtLib.Structures.Applicative.
 
 Require Import MirrorCharge.Java.Reify.
-Require Import MirrorCharge.Java.Syntax.
 
 Set Implicit Arguments.
 Set Strict Implicit.
@@ -53,24 +52,38 @@ Lemma rule_skip2 P G :(* P |-- Q -> *)G |-- {[P]} cskip {[P]}.
 Proof.
   apply rule_skip. reflexivity.
 Qed.
-	
+
+Notation "'ap_eq' '[' x ',' y ']'" :=
+	 (ap (T := Fun stack) (ap (T := Fun stack) (pure (T := Fun stack) (@eq sval)) x) y).
+Notation "'ap_pointsto' '[' x ',' f ',' e ']'" := 
+	(ap (T := Fun stack) (ap (T := Fun stack) (ap (T := Fun stack) 
+		(pure (T := Fun stack) pointsto) (stack_get x)) 
+			(pure (T := Fun stack) f)) e).
+Notation "'ap_typeof' '[' e ',' C ']'" :=
+	(ap (T := Fun stack) 
+	    (ap (T := Fun stack) 
+	        (pure (T := Fun stack) typeof) 
+	        (pure (T := Fun stack) C))
+	    e).
+
 Lemma rule_if (e : dexpr) c1 c2 (P Q : sasn) G
-      (Hc1 : G |-- {[(@embed (@vlogic String.string _) sasn _ 
-                      ap_eq [eval2 e, pure (T := Fun stack) (vbool true)]) //\\ P]} c1 {[Q]})
-      (Hc2 : G |-- {[(@embed (@vlogic String.string _) sasn _ 
-                      ap_eq [eval2 (E_not e), pure (T := Fun stack) (vbool true)]) //\\ P]} c2 {[Q]}) :
-  G |-- {[P]} cif e c1 c2 {[Q]}.
+      (Hc1 : G |-- {[(@embed (@vlogic var _) sasn _ 
+                      (ap_eq [eval e, pure (vbool true)])) //\\ P]} c1 {[Q]})
+      (Hc2 : G |-- {[(@embed (@vlogic var _) sasn _ 
+                      (ap_eq [eval (E_not e), pure (vbool true)])) //\\ P]} c2 {[Q]}) : 
+  G |-- {[P]} cif e c1 c2 {[Q]}. 
 Proof.
   eapply rule_if; unfold vlogic_eval, Open.liftn, Open.lift; simpl in *;
   	[apply Hc1|apply Hc2].
 Qed.
-
-  Lemma rule_read_fwd (x y : String.string) (f : String.string) (e : stack -> sval) (P Q : sasn) (G : spec)
-    (HP : P |-- ap (T := Fun stack) (ap (ap (pure pointsto2) (stack_get y)) (pure f)) e) 
-    (HQ : Exists v : sval, embed (ap_eq [stack_get x, apply_subst2 sval e (subst2 (pure v) x)]) //\\ 
-    					      (apply_subst2 asn P (subst2 (pure (T := Fun stack) v) x)) |-- Q) :
+Check @apply_subst.
+  Lemma rule_read_fwd (x y : var) (f : field) (e : stack -> sval) (P Q : sasn) (G : spec)
+    (HP : P |-- ap_pointsto [y, f, e])
+    (HQ : Exists v : sval, embed (ap_eq [stack_get x, apply_subst e (subst1 (pure (T := Fun stack) v) x)]) //\\ 
+    					      (apply_subst P (subst1 (pure (T := Fun stack) v) x)) |-- Q) :
     G |-- {[ P ]} cread x y f {[ Q ]}.
   Proof.
+    reify_imp (ap_pointsto [y, f, e]).
     pose proof @rule_read_fwd x y f e P. 
     unfold Open.liftn, Open.lift, open_eq, stack_get, Open.var_expr in *; simpl in *.
     rewrite <- HQ , <- H; [apply ltrueR | apply HP].
@@ -78,14 +91,14 @@ Qed.
 
 Require Import Charge.Logics.BILogic.
 
-  Lemma rule_write_fwd (x f : String.string) (e : dexpr) G (P Q F : sasn) (e' : stack -> sval)
+  Lemma rule_write_fwd (x : var) (f : field) (e : dexpr) G (P Q F : sasn) (e' : stack -> sval)
         (HP : P |-- ap_pointsto [x, f, e'] ** F) 
-        (HQ : ap_pointsto [x, f, eval2 e] ** F |-- Q) :
+        (HQ : ap_pointsto [x, f, eval e] ** F |-- Q) :
     G |-- ({[ P ]} cwrite x f e {[ Q ]}).
   Proof.
      pose proof @rule_write_frame G P F x f e' e. unfold Open.liftn, Open.lift, open_eq, stack_get, Open.var_expr in *; simpl in *.
 	 rewrite <- HQ, H.
-	 unfold stack. unfold pointsto2. unfold eval2.
+	 unfold stack. unfold pointsto. unfold eval.
 	 
 	 setoid_rewrite <- sepSPC1 at 2.
 	 reflexivity. 
@@ -94,11 +107,11 @@ Require Import Charge.Logics.BILogic.
 	 reflexivity.
   Qed.
 
-  Lemma rule_assign_fwd x (e : dexpr) G P :
+  Lemma rule_assign_fwd (x : var) (e : dexpr) G P :
     G |-- {[ P ]} cassign x e {[ Exists v : sval,
                                  embed (ap_eq [stack_get x, 
-                                               apply_subst2 sval (eval2 e) (subst2 (pure v) x)]) //\\ 
-    							   (apply_subst2 asn P (subst2 (pure (T := Fun stack) v) x)) ]}.
+                                               apply_subst (eval e) (subst1 (pure (T := Fun stack) v) x)]) //\\ 
+    							   (apply_subst P (subst1 (pure (T := Fun stack) v) x)) ]}.
   Proof.
     pose proof @rule_assign_fwd G P.
     apply H. reflexivity.
@@ -109,23 +122,23 @@ Definition set_fold_fun (x f : String.string) (P : sasn) :=
 
   Lemma rule_alloc_fwd (x C : String.string) (G : spec) (P : sasn) (fields : SS.t) (Pr : Prog_wf) 
 	(Heq : G |-- prog_eq Pr)
-	(Hf : field_lookup2 Pr C fields) :
+	(Hf : field_lookup Pr C fields) :
 	G |-- {[ P ]} calloc x C {[ Exists p : ptr, embed (ap_typeof [stack_get x, C] //\\
 	                                            ap_eq [stack_get x, pure (vptr p)]) //\\
 	                                            SS.fold (set_fold_fun x) fields 
-	                                                    (apply_subst2 asn P (subst2 (pure (T := Fun stack) p) x)) ]}.
+	                                                    (apply_subst P (subst1 (pure (T := Fun stack) p) x)) ]}.
   Proof.
   	admit.
   Qed.
 
 Require Import List.
-
+(*
   Lemma rule_static_complete C (m : String.string) (ps : list String.string) (es : list dexpr) (x r : var) G
     (P Q F Pm Qm : sasn)
-    (HSpec : G |-- |> method_spec2 C m ps r Pm Qm)
+    (HSpec : G |-- |> method_spec C m ps r Pm Qm)
     (HPre: P |-- apply_subst2 asn Pm (substl_trunc (zip ps (@map _ (stack -> sval) eval2 es))) ** F)
     (HLen: length ps = length es) :
-          G |-- {[ P ]} cscall x C m es {[ Exists v:sval, apply_subst2 asn Qm (substl_trunc (zip (@cons String.string r ps) 
+          G |-- {[ P ]} cscall x C m es {[ Exists v:sval, apply_subst asn Qm (substl_trunc (zip (@cons String.string r ps) 
                                      (@cons (stack -> sval) (stack_get x)
                                       (@map (stack -> sval) _ (fun e => apply_subst2 sval e (subst2 (pure (T := Fun stack) v) x)) 
                                           (@map dexpr (stack -> sval) eval2 es))))) ** 
@@ -156,3 +169,4 @@ Proof.
     assumption.
     reflexivity.
 Qed.
+*)
